Consistency proofs

candle/standard/semantics/holConsistencyScript.sml
@@ -7,13 +7,20 @@
 *)
 open preamble
      setSpecTheory holSyntaxLibTheory holSyntaxTheory holSyntaxExtraTheory holBoolSyntaxTheory holAxiomsSyntaxTheory
-     holSemanticsTheory holSemanticsExtraTheory holSoundnessTheory holExtensionTheory holBoolTheory holAxiomsTheory
+     holSemanticsTheory holSemanticsExtraTheory holSoundnessTheory holExtensionTheory holBoolTheory
 
 val _ = new_theory"holConsistency"
 
 val _ = Parse.hide "mem";
 
+val _ = Parse.hide "mem";
+
 val mem = ``mem:'U->'U->bool``
+
+Definition definitional_extension_def:
+  definitional_extension ctxt1 ctxt2 =
+    (ctxt1 extends ctxt2 /\ (!p. ~MEM (NewAxiom p) (TAKE (LENGTH ctxt1 - LENGTH ctxt2) ctxt1)))
+End
 
 val consistent_theory_def = Define`
   consistent_theory thy ⇔
@@ -22,7 +29,7 @@ val consistent_theory_def = Define`
 
 Theorem proves_consistent:
    is_set_theory ^mem ⇒
-    ∀thy. theory_ok thy ∧ (∃i. i models thy) ⇒
+    ∀thy. theory_ok thy ∧ (∃δ γ. models δ γ thy) ⇒
       consistent_theory thy
 Proof
   rw[consistent_theory_def] >- (
@@ -33,7 +40,7 @@ Proof
   spose_not_then strip_assume_tac >>
   imp_res_tac proves_sound >>
   fs[entails_def] >>
-  first_x_assum(qspecl_then[`δ`,`γ`]mp_tac) >>
+  first_x_assum drule >>
   simp[satisfies_def,satisfies_t_def] >>
   qexists_tac `K Bool` >>
   simp[tyvars_def] >>
@@ -83,12 +90,15 @@ Proof
   simp[boolean_eq_true,termsem_def,true_neq_false]
 QED
 
-val init_ctxt_builtin = Q.store_thm("init_ctxt_builtin",
-  `!ty. type_ok (tysof init_ctxt) ty /\ tyvars ty = [] ==> is_builtin_type ty`,
-  Cases >> rw[init_ctxt_def,type_ok_def,tyvars_def,is_builtin_type_def]);
+Theorem init_ctxt_builtin:
+  !ty. type_ok (tysof init_ctxt) ty /\ tyvars ty = [] ==> is_builtin_type ty
+Proof
+  Cases >> rw[init_ctxt_def,type_ok_def,tyvars_def,is_builtin_type_def]
+QED
 
-val init_ctxt_no_ground = Q.store_thm("init_ctxt_no_ground",
-`!ty. ty ∈ ground_types (sigof init_ctxt) ∩ nonbuiltin_types ==> F`,
+Theorem init_ctxt_no_ground:
+  !ty. ty ∈ ground_types (sigof init_ctxt) ∩ nonbuiltin_types ==> F'
+Proof
   ho_match_mp_tac type_ind >> rpt strip_tac
   >- fs[ground_types_def,tyvars_def]
   >> fs[ground_types_def,init_ctxt_def,tyvars_def]
@@ -96,15 +106,19 @@ val init_ctxt_no_ground = Q.store_thm("init_ctxt_no_ground",
   >> fs[type_ok_def]
   >> fs[EVERY_MEM,FLOOKUP_UPDATE]
   >> every_case_tac
-  >> rveq >> fs[nonbuiltin_types_def,is_builtin_type_def]);
+  >> rveq >> fs[nonbuiltin_types_def,is_builtin_type_def]
+QED
 
-val init_ctxt_no_ground_set = Q.store_thm("init_ctxt_no_ground_set",
-  `ground_types (sigof init_ctxt) ∩ nonbuiltin_types = {}`,
+Theorem init_ctxt_no_ground_set:
+  ground_types (sigof init_ctxt) ∩ nonbuiltin_types = {}
+Proof
   PURE_REWRITE_TAC [FUN_EQ_THM,EQ_IMP_THM,EMPTY_DEF] >> rpt strip_tac >>
-  metis_tac[init_ctxt_no_ground,IN_DEF]);
+  metis_tac[init_ctxt_no_ground,IN_DEF]
+QED
 
-val init_ctxt_has_model = Q.store_thm("init_ctxt_has_model",
-  `is_set_theory ^mem ⇒ ∃δ γ. models δ γ (thyof init_ctxt)`,
+Theorem init_ctxt_has_model:
+  is_set_theory ^mem ⇒ ∃δ γ. models δ γ (thyof init_ctxt)
+Proof
   rw[models_def,conexts_of_upd_def,total_fragment_def,
      is_frag_interpretation_def,init_ctxt_no_ground_set] >>
   MAP_EVERY qexists_tac [`ARB`,`ARB`] >>
@@ -116,176 +130,53 @@ val init_ctxt_has_model = Q.store_thm("init_ctxt_has_model",
      fs[ground_consts_def,term_ok_def,ELIM_UNCURRY,PULL_EXISTS] >>
      fs[init_ctxt_def,nonbuiltin_constinsts_def,builtin_consts_def] >>
      strip_tac >> Cases >> rw[]) >>
-  rw[is_type_frag_interpretation_def]);
+  rw[is_type_frag_interpretation_def]
+QED
 
 Theorem min_hol_consistent:
    is_set_theory ^mem ⇒
-    ∀ctxt. ctxt extends init_ctxt ∧ (∀p. MEM (NewAxiom p) ctxt ⇒ MEM (NewAxiom p) init_ctxt) ⇒
+    ∀ctxt. definitional_extension ctxt init_ctxt ∧
+      orth_ctxt ctxt ∧ terminating(subst_clos (dependency ctxt)) ⇒
       consistent_theory (thyof ctxt)
 Proof
+  simp[definitional_extension_def] >>
   strip_tac >> gen_tac >> strip_tac >>
   match_mp_tac (UNDISCH proves_consistent) >>
-  metis_tac[extends_theory_ok,extends_consistent,init_theory_ok,init_ctxt_has_model]
-QED
-
-val fhol_ctxt_def = Define`
-  fhol_ctxt = mk_select_ctxt (mk_eta_ctxt (mk_bool_ctxt init_ctxt))`
-
-Theorem fhol_extends_bool:
-   fhol_ctxt extends (mk_bool_ctxt init_ctxt)
-Proof
-  rw[fhol_ctxt_def] >>
-  match_mp_tac extends_trans >>
-  qexists_tac`mk_eta_ctxt (mk_bool_ctxt init_ctxt)` >>
-  reverse conj_asm2_tac >- (
-    match_mp_tac eta_extends >>
-    match_mp_tac is_bool_sig_std >>
-    match_mp_tac bool_has_bool_sig >>
-    `sigof init_ctxt = sigof (thyof init_ctxt)` by simp[] >>
-    metis_tac[theory_ok_sig,init_theory_ok] ) >>
-  match_mp_tac select_extends >>
-  EVAL_TAC
-QED
-
-fun tac extends_bool unfold =
-  strip_tac >> gen_tac >> strip_tac >>
-  assume_tac bool_extends_init >>
-  imp_res_tac init_ctxt_has_model >>
-  qspecl_then[`init_ctxt`,`mk_bool_ctxt init_ctxt`]mp_tac(UNDISCH extends_consistent) >>
-  simp[] >> disch_then(qspec_then`i`mp_tac) >>
-  simp[init_theory_ok] >>
-  impl_tac >- (EVAL_TAC >> simp[]) >>
-  disch_then(qx_choose_then`i2`strip_assume_tac) >>
-  qmatch_assum_abbrev_tac`ctxt extends ctxt0` >>
-  `theory_ok (thyof ctxt0)` by (
-    match_mp_tac (MP_CANON extends_theory_ok) >>
-    qexists_tac`init_ctxt` >>
-    metis_tac[init_theory_ok,extends_bool,bool_extends_init,extends_trans]) >>
-  qunabbrev_tac`ctxt0` >>
-  conj_asm1_tac >- (
-    match_mp_tac (MP_CANON extends_theory_ok) >>
-    metis_tac[]) >>
-  unfold >>
-  qspec_then`mk_bool_ctxt init_ctxt`mp_tac(UNDISCH eta_has_model) >>
-  `∀ctxt. sigof ctxt = sigof (thyof ctxt)` by simp[] >>
-  impl_tac >- (
-    match_mp_tac is_bool_sig_std >>
-    match_mp_tac bool_has_bool_sig >>
-    metis_tac[theory_ok_sig,init_theory_ok] ) >>
-  disch_then(qspec_then`i2`mp_tac) >> simp[] >> strip_tac >>
-  qspec_then`mk_eta_ctxt (mk_bool_ctxt init_ctxt)`mp_tac(UNDISCH select_has_model) >>
-  `theory_ok (thyof (mk_eta_ctxt (mk_bool_ctxt init_ctxt)))` by (
-    match_mp_tac (MP_CANON extends_theory_ok) >>
-    qexists_tac`mk_bool_ctxt init_ctxt` >>
-    reverse conj_asm2_tac >-
-      metis_tac[extends_theory_ok,bool_extends_init,init_theory_ok] >>
-    match_mp_tac eta_extends >>
-    metis_tac[theory_ok_sig] ) >>
-  impl_tac >- ( rw[] >> EVAL_TAC ) >>
-  disch_then(qspec_then`i2`mp_tac) >>
-  qspecl_then[`init_ctxt`,`i2`]mp_tac(UNDISCH bool_has_bool_interpretation) >>
-  impl_tac >- (
-    metis_tac[extends_theory_ok,bool_extends_init,init_theory_ok] ) >>
-  strip_tac >>
-  impl_tac >- fs[is_bool_interpretation_def] >>
-  disch_then(qx_choose_then`i3`strip_assume_tac)
-
-Theorem fhol_has_model:
-   is_set_theory ^mem ⇒
-    ∀ctxt.
-      ctxt extends fhol_ctxt ∧
-      (∀p. MEM (NewAxiom p) ctxt ⇒ MEM (NewAxiom p) fhol_ctxt) ⇒
-      theory_ok (thyof ctxt) ∧ ∃i. i models thyof ctxt
-Proof
-  tac fhol_extends_bool ALL_TAC >>
-  fs[GSYM fhol_ctxt_def] >>
-  qspecl_then[`fhol_ctxt`,`ctxt`]mp_tac(UNDISCH extends_consistent) >> simp[] >>
+  assume_tac init_theory_ok >>
+  imp_res_tac extends_theory_ok >>
+  drule min_hol_interpretation_is_model >>
+  ntac 3 (disch_then drule) >>
+  impl_tac >-
+    (imp_res_tac extends_appends >> fs[TAKE_APPEND,init_ctxt_def]) >>
   metis_tac[]
 QED
 
-Theorem fhol_consistent:
+Theorem finite_hol_consistent:
    is_set_theory ^mem ⇒
-    ∀ctxt.
-      ctxt extends fhol_ctxt ∧
-      (∀p. MEM (NewAxiom p) ctxt ⇒ MEM (NewAxiom p) fhol_ctxt) ⇒
+    ∀ctxt. definitional_extension ctxt finite_hol_ctxt ∧
+      orth_ctxt ctxt ∧ terminating(subst_clos (dependency ctxt)) ⇒
       consistent_theory (thyof ctxt)
 Proof
+  simp[definitional_extension_def] >>
   strip_tac >> gen_tac >> strip_tac >>
   match_mp_tac (UNDISCH proves_consistent) >>
-  metis_tac[fhol_has_model]
-QED
-
-val hol_ctxt_def = Define`
-  hol_ctxt = mk_infinity_ctxt fhol_ctxt`
-
-Theorem hol_extends_fhol:
-   hol_ctxt extends fhol_ctxt
-Proof
-  rw[hol_ctxt_def] >>
-  match_mp_tac infinity_extends >>
-  reverse conj_tac >- EVAL_TAC >>
-  match_mp_tac (MP_CANON extends_theory_ok) >>
-  match_exists_tac (concl fhol_extends_bool) >>
-  conj_tac >- ACCEPT_TAC fhol_extends_bool >>
-  match_mp_tac (MP_CANON extends_theory_ok) >>
-  metis_tac[bool_extends_init,init_theory_ok]
-QED
-
-Theorem hol_extends_bool:
-   hol_ctxt extends (mk_bool_ctxt init_ctxt)
-Proof
-  match_mp_tac extends_trans >>
-  metis_tac[hol_extends_fhol,fhol_extends_bool]
-QED
-
-Theorem hol_has_model:
-   is_set_theory ^mem ∧ (∃inf. is_infinite ^mem inf) ⇒
-    ∀ctxt.
-      ctxt extends hol_ctxt ∧
-      (∀p. MEM (NewAxiom p) ctxt ⇒ MEM (NewAxiom p) hol_ctxt) ⇒
-      theory_ok (thyof ctxt) ∧ ∃i. i models thyof ctxt
-Proof
-  tac hol_extends_bool (fs[hol_ctxt_def]) >>
-  assume_tac(UNDISCH(PROVE[]``is_infinite mem inf ⇒ ∃inf. is_infinite ^mem inf``)) >>
-  qspec_then`mk_select_ctxt (mk_eta_ctxt (mk_bool_ctxt init_ctxt))`mp_tac
-    (infinity_has_model |> ONCE_REWRITE_RULE[GSYM AND_IMP_INTRO] |> UNDISCH |> UNDISCH) >>
-  pop_assum kall_tac >>
-  impl_tac >- (
-    conj_tac >- (
-      match_mp_tac (MP_CANON extends_theory_ok) >>
-      qexists_tac`mk_eta_ctxt (mk_bool_ctxt init_ctxt)` >>
-      conj_tac >- (
-        match_mp_tac select_extends >>
-        imp_res_tac theory_ok_sig >> fs[] >>
-        EVAL_TAC ) >>
-      simp[] ) >>
-    EVAL_TAC ) >>
-  disch_then(qspec_then`i3`mp_tac) >>
-  impl_tac >- (
-    simp[] >>
-    fs[is_bool_interpretation_def] >>
-    fs[is_implies_interpretation_def,is_and_interpretation_def,is_forall_interpretation_def,
-       is_exists_interpretation_def,is_not_interpretation_def] >>
-    rpt conj_tac >>
-    match_mp_tac equal_on_interprets >>
-    map_every qexists_tac[`sigof(mk_eta_ctxt (mk_bool_ctxt init_ctxt))`,`i2`] >> simp[] >>
-    EVAL_TAC >> simp[] >> EVAL_TAC >> simp[SUBSET_DEF] ) >>
-  disch_then(qx_choose_then`i4`strip_assume_tac) >>
-  fs[GSYM hol_ctxt_def,GSYM fhol_ctxt_def] >>
-  qspecl_then[`hol_ctxt`,`ctxt`]mp_tac(UNDISCH extends_consistent) >> simp[] >>
-  metis_tac[]
+  assume_tac init_theory_ok >>
+  metis_tac[extends_theory_ok,finite_hol_interpretation_is_model,
+            extends_trans,finite_hol_ctxt_extends_init]
 QED
 
 Theorem hol_consistent:
-   is_set_theory ^mem ∧ (∃inf. is_infinite ^mem inf) ⇒
-    ∀ctxt.
-      ctxt extends hol_ctxt ∧
-      (∀p. MEM (NewAxiom p) ctxt ⇒ MEM (NewAxiom p) hol_ctxt) ⇒
+   is_set_theory ^mem /\ is_infinite ^mem ind ⇒
+    ∀ctxt. definitional_extension ctxt hol_ctxt ∧
+      orth_ctxt ctxt ∧ terminating(subst_clos (dependency ctxt)) ⇒
       consistent_theory (thyof ctxt)
 Proof
+  simp[definitional_extension_def] >>
   strip_tac >> gen_tac >> strip_tac >>
   match_mp_tac (UNDISCH proves_consistent) >>
-  metis_tac[hol_has_model]
+  assume_tac init_theory_ok >>
+  metis_tac[extends_theory_ok,hol_interpretation_is_model,
+            extends_trans,hol_ctxt_extends_init]
 QED
 
 val _ = export_theory()
